feat: update the date calculation logic into using external libraries

DateTimeImpl.cs
@@ -1,0 +1,53 @@
+using System;
+using System.Linq;
+using System.Numerics;
+using Dafny;
+
+public static class DateTimeImpl
+{
+    public static ISequence<Rune> GetNowComponents()
+    {
+        var now = DateTime.Now;
+        var components = new[] {
+            now.Year,
+            now.Month,
+            now.Day,
+            now.Hour,
+            now.Minute,
+            now.Second,
+            now.Millisecond
+        };
+
+        // Convert to sequence of integers as runes
+        var runes = components.Select(i => new Rune(i)).ToArray();
+        return Sequence<Rune>.FromArray(runes);
+    }
+
+    public static BigInteger ToEpochTimeMilliseconds(BigInteger year, BigInteger month, BigInteger day, BigInteger hour, BigInteger minute, BigInteger second, BigInteger millisecond, TimeSpan? offset = null)
+    {
+        return new DateTimeOffset((int)year, (int)month, (int)day, (int)hour, (int)minute, (int)second, (int)millisecond, offset ?? TimeSpan.Zero)
+            .ToUnixTimeMilliseconds();
+    }
+
+    public static ISequence<BigInteger> FromEpochTimeMilliseconds(BigInteger epochMilliseconds, TimeSpan? offset = null)
+    {
+        DateTimeOffset dateTimeOffset = DateTimeOffset.FromUnixTimeMilliseconds((long)epochMilliseconds)
+            .ToOffset(offset ?? TimeSpan.Zero);
+        var components = new BigInteger[]
+        {
+            dateTimeOffset.Year,
+            dateTimeOffset.Month,
+            dateTimeOffset.Day,
+            dateTimeOffset.Hour,
+            dateTimeOffset.Minute,
+            dateTimeOffset.Second,
+            dateTimeOffset.Millisecond
+        };
+        return Sequence<BigInteger>.FromArray(components);
+    }
+
+    public static bool IsLeapYear(BigInteger year)
+    {
+        return DateTime.IsLeapYear((int)year);
+    }
+}
